last exercise

analysis/Analysis/Section_3_5.lean
@@ -52,12 +52,66 @@ theorem OrderedPair.eq (x y x' y' : Object) :
 /-- Helper lemma for Exercise 3.5.1 -/
 lemma SetTheory.Set.pair_eq_singleton_iff {a b c: Object} : {a, b} = ({c}: Set) ↔
     a = c ∧ b = c := by
-  sorry
+      constructor
+      . 
+        intro h
+        simp[SetTheory.Set.ext_iff] at h
+        have hac := h a
+        have hbc := h b
+        tauto 
+      intro ⟨hac, hbc⟩ 
+      ext x
+      rw[hac,hbc]
+      simp
+
+lemma SetTheory.Set.singleton_eq_singleton_iff {a b:Object} : {a} = ({b} : Set) ↔ a = b := by
+  constructor
+  . 
+    intro h
+    rw[SetTheory.Set.ext_iff] at h
+    specialize h a
+    simp at h
+    exact h
+  intro h
+  rw[h]
+
+lemma SetTheory.Set.singleton_eq_pair_iff {a b c:Object} :{c} = ({a,b}:Set) ↔ a = c ∧ b = c := by
+  rw[← pair_eq_singleton_iff]
+  constructor <;> intro h <;> symm <;> exact h
+
+lemma SetTheory.Set.pair_eq_pair_iff {a b c d:Object} :  
+    ({a,b}:Set) = {c,d} ↔ a = c ∧ b = d ∨ a = d ∧ b = c := by
+      constructor
+      .
+        intro h
+        exact pair_eq_pair h
+      rintro (⟨h1, h2⟩|⟨h1,h2⟩ ) 
+      <;> rw[h1,h2]
+      ext x
+      simp
+      tauto
 
 /-- Exercise 3.5.1, first part -/
 def OrderedPair.toObject : OrderedPair ↪ Object where
   toFun p := ({ (({p.fst}:Set):Object), (({p.fst, p.snd}:Set):Object) }:Set)
-  inj' := by sorry
+  inj' := by
+    simp[Function.Injective]
+    intro p1 p2
+    intro h12
+    simp[SetTheory.Set.ext_iff] at h12
+    have ffst := h12 (({p1.fst}:Set):Object)
+    simp at ffst
+    have fsnd := h12 (SetTheory.set_to_object {p1.fst, p1.snd})
+    simp at fsnd
+    obtain (hfstA| hfstB) := ffst <;>
+    obtain (hsndA | hsndB) := fsnd <;>
+    ext 
+    all_goals
+      simp_all [singleton_eq_singleton_iff, pair_eq_singleton_iff, singleton_eq_pair_iff,pair_eq_pair_iff]
+    obtain (h1|h2) := hsndB
+    tauto
+    have ⟨h21,h22⟩ := h2
+    simp_all
 
 instance OrderedPair.inst_coeObject : Coe OrderedPair Object where
   coe := toObject
@@ -152,10 +206,16 @@ example : ({1, 2}: Set) ×ˢ ({3, 4, 5}: Set) = ({
 
 /-- Example 3.5.5 / Exercise 3.6.5. There is a bijection between `X ×ˢ Y` and `Y ×ˢ X`. -/
 noncomputable abbrev SetTheory.Set.prod_commutator (X Y:Set) : X ×ˢ Y ≃ Y ×ˢ X where
-  toFun := sorry
-  invFun := sorry
-  left_inv := sorry
-  right_inv := sorry
+  toFun := fun z ↦ 
+  ⟨(⟨ snd z, fst z⟩:OrderedPair) , by simp ⟩  
+  invFun := fun z ↦ 
+  ⟨(⟨ snd z, fst z⟩:OrderedPair) , by simp ⟩  
+  left_inv z := by
+    rw[← mk_cartesian_fst_snd_eq z,mk_cartesian ]
+    simp
+  right_inv z := by
+    rw[← mk_cartesian_fst_snd_eq z,mk_cartesian ]
+    simp
 
 /-- Example 3.5.5. A function of two variables can be thought of as a function of a pair. -/
 noncomputable abbrev SetTheory.Set.curry_equiv {X Y Z:Set} : (X → Y → Z) ≃ (X ×ˢ Y → Z) where
@@ -167,10 +227,21 @@ noncomputable abbrev SetTheory.Set.curry_equiv {X Y Z:Set} : (X → Y → Z) ≃
 /-- Definition 3.5.6.  The indexing set `I` plays the role of `{ i : 1 ≤ i ≤ n }` in the text.
     See Exercise 3.5.10 below for some connections betweeen this concept and the preceding notion
     of Cartesian product and ordered pair.  -/
+-- tuple is essentially a function
+-- x is I → X indeed, hence ,given i, choose a element xᵢ  in Xᵢ 
+-- so the tuple itself is an objectified function which 
+-- takes x, wrapped it, change the return type from subType Xᵢ to subType (Bigunion of Xᵢ's)
+-- it can also be seen as a series T, Tᵢ is `tuple x i`
+
+
 abbrev SetTheory.Set.tuple {I:Set} {X: I → Set} (x: ∀ i, X i) : Object :=
   ((fun i ↦ ⟨ x i, by rw [mem_iUnion]; use i; exact (x i).property ⟩):I → iUnion I X)
 
+
 /-- Definition 3.5.6 -/
+-- before specification, it's all possible functions mapping i to all possible elements in bigUnion Xᵢ 
+-- after that ,i can only map to elements in Xᵢ but still as a subtype of the bigunion
+
 abbrev SetTheory.Set.iProd {I: Set} (X: I → Set) : Set :=
   ((iUnion I X)^I).specify (fun t ↦ ∃ x : ∀ i, X i, t = tuple x)
 
@@ -188,7 +259,17 @@ theorem SetTheory.Set.tuple_mem_iProd {I: Set} {X: I → Set} (x: ∀ i, X i) :
 
 @[simp]
 theorem SetTheory.Set.tuple_inj {I:Set} {X: I → Set} (x y: ∀ i, X i) :
-    tuple x = tuple y ↔ x = y := by sorry
+    tuple x = tuple y ↔ x = y := by
+      constructor
+      . 
+        simp
+        intro hf
+        ext i
+        have hp:=congrArg (fun f => f i) hf 
+        simp at hp
+        exact hp
+      intro h
+      rw[h]
 
 /-- Example 3.5.8. There is a bijection between `(X ×ˢ Y) ×ˢ Z` and `X ×ˢ (Y ×ˢ Z)`. -/
 noncomputable abbrev SetTheory.Set.prod_associator (X Y Z:Set) : (X ×ˢ Y) ×ˢ Z ≃ X ×ˢ (Y ×ˢ Z) where
@@ -203,41 +284,176 @@ noncomputable abbrev SetTheory.Set.prod_associator (X Y Z:Set) : (X ×ˢ Y) ×ˢ
 -/
 noncomputable abbrev SetTheory.Set.singleton_iProd_equiv (i:Object) (X:Set) :
     iProd (fun _:({i}:Set) ↦ X) ≃ X where
-  toFun := sorry
-  invFun := sorry
-  left_inv := sorry
-  right_inv := sorry
+  toFun tup := (((mem_iProd _).mp tup.property).choose) ⟨i, by simp⟩ 
+  invFun x :=  ⟨tuple (fun _ ↦ x),by rw[mem_iProd] ;use (fun _ ↦ x)⟩ 
+  left_inv tup := by
+    have spec :=(((mem_iProd _).mp tup.property).choose_spec) 
+    ext
+    rw[spec,tuple_inj]
+    simp
+    funext i'
+    have : i' = ⟨i, by simp⟩ := by
+      have := i'.property
+      simp at this
+      ext
+      simp
+      exact this
+    rw[this]
+  right_inv x := by
+    simp
+    generalize_proofs ex hi
+    have spec := ex.choose_spec
+    rw[tuple_inj] at spec
+    simp [← spec]
+
+abbrev SetTheory.Set.empty_tuple  {X: (∅:Set)  → Set}  : iProd X := 
+  let fx : (i : (∅ : Set)) → (X i) := by
+      intro ⟨i, hi⟩ 
+      simp at hi
+  ⟨ tuple fx, by simp; use fx⟩ 
+lemma SetTheory.Set.unique_empty_tuple {X: (∅:Set)  → Set}  { f  : iProd X } : f = empty_tuple := by
+  obtain ⟨f, hf⟩ := f 
+  obtain ⟨h1, rfl⟩ := (mem_iProd _).mp hf 
+  rw[empty_tuple]
+  congr
+  funext x
+  obtain ⟨x, hx⟩ := x
+  simp at hx
 
 /-- Example 3.5.10 -/
 abbrev SetTheory.Set.empty_iProd_equiv (X: (∅:Set) → Set) : iProd X ≃ Unit where
-  toFun := sorry
-  invFun := sorry
-  left_inv := sorry
-  right_inv := sorry
+  toFun := (fun tup ↦ PUnit.unit)
+  invFun := fun u ↦ empty_tuple  
+  left_inv tup := by
+    simp
+    exact unique_empty_tuple.symm
+  right_inv x := by
+    simp
 
 /-- Example 3.5.10 -/
 noncomputable abbrev SetTheory.Set.iProd_of_const_equiv (I:Set) (X: Set) :
     iProd (fun i:I ↦ X) ≃ (I → X) where
-  toFun := sorry
-  invFun := sorry
-  left_inv := sorry
-  right_inv := sorry
+  toFun prod := 
+      ((mem_iProd _).mp (prod.property)).choose
+  invFun x := ⟨tuple fun i:I ↦ (x i), tuple_mem_iProd fun i:I ↦ (x i) ⟩ 
+  left_inv prod := by
+    have spec := ((mem_iProd _).mp prod.property).choose_spec
+    ext
+    simp[← spec]
+  right_inv x := by
+    simp
+    generalize_proofs hxi hxi2 ht
+    have spec := ht.choose_spec
+    funext i
+    ext 
+    have t := congrArg (fun f => f i) spec
+    simp at t
+    simp[t]
+open Classical in
+noncomputable def SetTheory.Set.cartesian_to_tuple_fx {X: ({0,1}:Set) → Set}
+  (pair : (X ⟨0, by simp⟩ ×ˢ X ⟨1, by simp⟩)) : (i: ({0,1}:Set)) → X i := 
+    fun ⟨i, hi⟩ =>
+      if h : i = 0
+        then ⟨fst pair, by simp[h, (fst pair).property]⟩ 
+        else ⟨snd pair, by simp[h]at hi; simp[hi, (snd pair).property]⟩  
 
+lemma SetTheory.Set.cartesian_to_tuple_fx_eq {X: ({0,1}:Set) → Set}
+  {x : ∀ i, X i} : 
+  cartesian_to_tuple_fx (mk_cartesian (x ⟨0, by simp⟩) (x ⟨1, by simp⟩)) = x := by
+    unfold cartesian_to_tuple_fx
+    funext i
+    by_cases hi : i = ⟨0, by simp⟩ 
+    . 
+      aesop
+    have hi' : i = ⟨ 1, by simp⟩ := by
+      aesop
+    aesop
 /-- Example 3.5.10 -/
 noncomputable abbrev SetTheory.Set.iProd_equiv_prod (X: ({0,1}:Set) → Set) :
     iProd X ≃ (X ⟨ 0, by simp ⟩) ×ˢ (X ⟨ 1, by simp ⟩) where
-  toFun := sorry
-  invFun := sorry
-  left_inv := sorry
-  right_inv := sorry
+  toFun prod := 
+     mk_cartesian (((mem_iProd _).mp prod.property).choose ⟨0, by simp⟩ ) (((mem_iProd _).mp prod.property).choose ⟨1, by simp⟩ )
+  invFun pair :=     
+    ⟨ tuple (cartesian_to_tuple_fx pair) ,  tuple_mem_iProd (cartesian_to_tuple_fx pair)⟩
+  left_inv prod := by
+    have ⟨pv, hp⟩ := prod 
+    rw[mem_iProd] at hp
+    have spec := hp.choose_spec
+    simp
+    conv_rhs => rw[spec]
+    rw[tuple_inj]
+    exact cartesian_to_tuple_fx_eq 
+  right_inv pair := by
+    set fx := cartesian_to_tuple_fx pair with hfx
+    set tup := tuple fx with htup
+    set prod :iProd X := ⟨tup, tuple_mem_iProd fx ⟩ with hprod
+    have spec := ((mem_iProd _).mp prod.property).choose_spec
+    change  mk_cartesian (((mem_iProd _).mp prod.property).choose ⟨0, by simp⟩ ) (((mem_iProd _).mp prod.property).choose ⟨1, by simp⟩ ) = pair
+    simp[hprod] at spec
+    conv_lhs at spec => rw[htup]
+    rw[tuple_inj] at spec
+    rw[← spec]
+    simp[fx,cartesian_to_tuple_fx]
+open Classical in
+noncomputable def SetTheory.Set.cartesian_to_triple_fx {X: ({0,1,2}:Set) → Set}
+  (pair : (X ⟨0, by simp⟩ ×ˢ X ⟨1, by simp⟩ ×ˢ X ⟨2, by simp⟩ )) : (i: ({0,1,2}:Set)) → X i := 
+    fun ⟨i, hi⟩ =>
+      if h : i = 0
+        then ⟨fst pair, by simp[h, (fst pair).property]⟩ 
+        else if h' : i = 1 
+          then ⟨fst (snd pair), by simp [h' , (fst (snd pair)).property]⟩ 
+          else ⟨snd (snd pair), by simp[h,h']at hi; simp[hi, (snd (snd pair)).property]⟩  
+
+lemma SetTheory.Set.cartesian_to_triple_fx_eq {X: ({0,1,2}:Set) → Set}
+  {x : ∀ i, X i} : 
+  cartesian_to_triple_fx (mk_cartesian (x ⟨0, by simp⟩) (mk_cartesian (x ⟨1, by simp⟩) (x ⟨2, by simp⟩))) = x := by
+    unfold cartesian_to_triple_fx
+    funext i
+    by_cases hi : i = ⟨0, by simp⟩ 
+    . 
+      aesop
+    by_cases hi' : i = ⟨1, by simp⟩ 
+    .
+      aesop
+    have hi'' : i = ⟨2 , by simp⟩ := by
+      aesop
+    aesop
+
 
 /-- Example 3.5.10 -/
 noncomputable abbrev SetTheory.Set.iProd_equiv_prod_triple (X: ({0,1,2}:Set) → Set) :
     iProd X ≃ (X ⟨ 0, by simp ⟩) ×ˢ (X ⟨ 1, by simp ⟩) ×ˢ (X ⟨ 2, by simp ⟩) where
-  toFun := sorry
-  invFun := sorry
-  left_inv := sorry
-  right_inv := sorry
+  toFun prod := 
+     mk_cartesian (((mem_iProd _).mp prod.property).choose ⟨0, by simp⟩ ) (
+      mk_cartesian 
+      (((mem_iProd _).mp prod.property).choose ⟨1, by simp⟩ )
+      (((mem_iProd _).mp prod.property).choose ⟨2, by simp⟩ )
+    )
+  invFun pair := 
+     ⟨ tuple (cartesian_to_triple_fx pair) ,  tuple_mem_iProd (cartesian_to_triple_fx pair)⟩
+  left_inv prod := by
+    have ⟨pv, hp⟩ := prod 
+    rw[mem_iProd] at hp
+    have spec := hp.choose_spec
+    simp
+    conv_rhs => rw[spec]
+    rw[tuple_inj]
+    exact cartesian_to_triple_fx_eq 
+  right_inv pair := by
+    set fx := cartesian_to_triple_fx pair with hfx
+    set tup := tuple fx with htup
+    set prod :iProd X := ⟨tup, tuple_mem_iProd fx ⟩ with hprod
+    have spec := ((mem_iProd _).mp prod.property).choose_spec
+    change mk_cartesian (((mem_iProd _).mp prod.property).choose ⟨0, by simp⟩ ) (
+      mk_cartesian 
+      (((mem_iProd _).mp prod.property).choose ⟨1, by simp⟩ )
+      (((mem_iProd _).mp prod.property).choose ⟨2, by simp⟩ )
+    ) = pair
+    simp[hprod] at spec
+    conv_lhs at spec => rw[htup]
+    rw[tuple_inj] at spec
+    rw[← spec]
+    simp[fx,cartesian_to_triple_fx]
 
 /-- Connections with Mathlib's `Set.pi` -/
 noncomputable abbrev SetTheory.Set.iProd_equiv_pi (I:Set) (X: I → Set) :
@@ -365,7 +581,44 @@ theorem SetTheory.Set.finite_choice {n:ℕ} {X: Fin n → Set} (h: ∀ i, X i �
 /-- Exercise 3.5.1, second part (requires axiom of regularity) -/
 abbrev OrderedPair.toObject' : OrderedPair ↪ Object where
   toFun p := ({ p.fst, (({p.fst, p.snd}:Set):Object) }:Set)
-  inj' := by sorry
+  inj' p1 p2 := by
+    intro h12
+    simp[SetTheory.Set.ext_iff] at h12
+    have ffst := h12 p1.fst
+    simp at ffst
+    have fsnd := h12 ( ({p1.fst, p1.snd} : Set) :Object)
+    simp at fsnd
+    obtain (feq|fother) := ffst
+    <;> obtain (sother|seq) := fsnd
+    . 
+      rw[feq] at sother
+      have con := not_mem_self ({p2.fst,p1.snd})
+      rw[sother] at con
+      simp at con
+    . 
+      ext
+      . exact feq
+      rw[feq]at seq
+      have cases := pair_eq_pair seq
+      simp at cases
+      obtain (case1 | ⟨case2_1 , case2_2⟩  ) := cases
+      . tauto
+      rw[case2_2]
+      exact case2_1
+    .
+      have con := not_mem_mem  {p2.fst,p2.snd} {p1.fst, p1.snd}
+      obtain (case1 | case2 ) := con
+      .
+        simp[← fother] at case1
+      simp[← sother] at case2
+    .
+      have cases := pair_eq_pair seq
+      simp at cases
+      obtain (⟨case1,case12⟩|⟨case1,case22⟩) := cases  
+      all_goals
+        rw[case1] at fother
+        have con := not_mem_self ({p2.fst,p2.snd})
+        simp [←fother] at con
 
 /-- An alternate definition of a tuple, used in Exercise 3.5.2 -/
 structure SetTheory.Set.Tuple (n:ℕ) where
@@ -387,115 +640,712 @@ lemma SetTheory.Set.Tuple.ext {n:ℕ} {t t':Tuple n}
 
 /-- Exercise 3.5.2 -/
 theorem SetTheory.Set.Tuple.eq {n:ℕ} (t t':Tuple n) :
-    t = t' ↔ ∀ n : Fin n, ((t.x n):Object) = ((t'.x n):Object) := by sorry
-
+    t = t' ↔ ∀ n : Fin n, ((t.x n):Object) = ((t'.x n):Object) := by
+      constructor
+      . 
+        intro eq m
+        rw[eq]
+      intro eq
+      ext u
+      .
+        constructor
+        <;> intro memt
+        map_tacs[have surj := t.surj; have surj := t'.surj]
+        all_goals
+          unfold Function.Surjective at surj
+          specialize surj ⟨u, memt⟩ 
+          obtain ⟨a, ha⟩ := surj 
+          specialize eq a
+          rw[ha] at eq
+          simp at eq
+        map_tacs[have prop := (t'.x a).property; have prop := (t.x a).property]
+        . simp[eq]; exact prop
+        simp[← eq]; exact prop  
+      exact eq u
 noncomputable abbrev SetTheory.Set.iProd_equiv_tuples (n:ℕ) (X: Fin n → Set) :
     iProd X ≃ { t:Tuple n // ∀ i, (t.x i:Object) ∈ X i } where
-  toFun := sorry
-  invFun := sorry
-  left_inv := sorry
-  right_inv := sorry
+  toFun prod := by
+    set fx := ( (mem_iProd _).mp prod.property ).choose with hfx
+    set codom :Set := (iUnion (Fin n) X).specify (fun a ↦ ∃ m, a.val = fx m)  with hcod
+    set f : Fin n → codom := fun i ↦ ⟨
+      fx i, 
+      by 
+        rw[hcod,specification_axiom'']
+        have h : (fx i).val ∈ (Fin n).iUnion X := by
+          rw[mem_iUnion]
+          use i
+          exact (fx i).property
+        use h,i
+    ⟩ 
+    exact ⟨⟨codom, f, by 
+      unfold Function.Surjective 
+      intro b
+      simp_all [fx, codom, f]
+      obtain ⟨val, property⟩ := prod
+      obtain ⟨val_1, property_1⟩ := b
+      simp_all only [Subtype.mk.injEq, codom, fx]
+      simp_all [codom, fx]
+      obtain ⟨left, right⟩ := property_1
+      obtain ⟨w, h⟩ := right
+      obtain ⟨w_1, h⟩ := h
+      obtain ⟨w_1, h⟩ := w_1
+      subst h
+      apply Exists.intro
+      · apply Exists.intro
+        · rfl
+        · simp_all only [exists_const]
+    ⟩ 
+,by 
+      grind only [cases eager Subtype]
+    ⟩ 
+  invFun tup := by
+    obtain ⟨tup, htup⟩ := tup 
+    have f : ∀ i, X i := fun i ↦ ⟨ tup.x i, htup i⟩  
+    exact ⟨tuple f, tuple_mem_iProd f⟩ 
+  left_inv prod := by
+    simp only [Subtype.coe_eta]
+    have hfx := ( (mem_iProd _).mp prod.property ).choose_spec 
+    ext
+    conv_rhs => rw[hfx]
+
+  right_inv tup := by
+    obtain ⟨tup , htup⟩ := tup 
+    set f : ∀ i, X i := fun i ↦ ⟨ tup.x i, htup i⟩ with hf
+    set prod: iProd X := ⟨tuple f, tuple_mem_iProd f⟩ with hprod
+    set fx := ( (mem_iProd _).mp prod.property ).choose with hfx
+    have spec := ( (mem_iProd _).mp prod.property ).choose_spec
+    rw[hprod] at spec
+    rw[tuple_inj] at spec
+    
+    simp only [Lean.Elab.WF.paramLet, Subtype.mk.injEq]
+    ext t
+    . 
+      simp only [Subtype.exists, specification_axiom'', exists_prop]
+      constructor
+      .
+        intro ht
+        obtain ⟨ht, ⟨a,⟨ha, hfin⟩ ,h⟩ ⟩ := ht 
+        rw[h]
+        rw[← spec]
+        simp[f]
+        have xp := (tup.x (⟨a, by simp; use ha ⟩) ).property
+        exact xp
+      intro ht
+      have surj := tup.surj
+      unfold Function.Surjective at surj
+      specialize surj ⟨t,ht⟩ 
+      obtain ⟨a, hxi⟩ := surj 
+      split_ands
+      .
+        specialize htup a
+        simp[hxi] at htup
+        rw[mem_iUnion]
+        use a
+      use a.val
+      have ap := a.property
+      simp at ap
+      use ap
+      simp[← spec,f,hxi]
+    . 
+      simp[← spec,f]
 
 /--
   Exercise 3.5.3. The spirit here is to avoid direct rewrites (which make all of these claims
   trivial), and instead use `OrderedPair.eq` or `SetTheory.Set.tuple_inj`
 -/
-theorem OrderedPair.refl (p: OrderedPair) : p = p := by sorry
+theorem OrderedPair.refl (p: OrderedPair) : p = p := by 
+  rw[OrderedPair.eq]
+  split_ands <;> rfl
+  
 
-theorem OrderedPair.symm (p q: OrderedPair) : p = q ↔ q = p := by sorry
+theorem OrderedPair.symm (p q: OrderedPair) : p = q ↔ q = p := by
+  constructor
+  <;> intro h
+  <;> rw[OrderedPair.eq] at *
+  <;> obtain ⟨h1, h2⟩ := h  
+  <;> tauto
 
-theorem OrderedPair.trans {p q r: OrderedPair} (hpq: p=q) (hqr: q=r) : p=r := by sorry
+theorem OrderedPair.trans {p q r: OrderedPair} (hpq: p=q) (hqr: q=r) : p=r := by
+  rw[OrderedPair.eq] at *
+  obtain ⟨fpq,spq⟩ := hpq
+  obtain ⟨fqr,sqr⟩ := hqr
+  rw[fqr]at fpq
+  rw[sqr]at spq
+  tauto
 
 theorem SetTheory.Set.tuple_refl {I:Set} {X: I → Set} (a: ∀ i, X i) :
-    tuple a = tuple a := by sorry
+    tuple a = tuple a := by 
+    rw[tuple_inj]
+
 
 theorem SetTheory.Set.tuple_symm {I:Set} {X: I → Set} (a b: ∀ i, X i) :
-    tuple a = tuple b ↔ tuple b = tuple a := by sorry
+    tuple a = tuple b ↔ tuple b = tuple a := by
+      constructor
+      <;> intro h
+      <;> rw[tuple_inj] at *
+      <;> exact h.symm
 
 theorem SetTheory.Set.tuple_trans {I:Set} {X: I → Set} {a b c: ∀ i, X i}
   (hab: tuple a = tuple b) (hbc : tuple b = tuple c) :
-    tuple a = tuple c := by sorry
+    tuple a = tuple c := by
+      rw[tuple_inj] at *
+      rw[hbc]at hab
+      exact hab
 
 /-- Exercise 3.5.4 -/
-theorem SetTheory.Set.prod_union (A B C:Set) : A ×ˢ (B ∪ C) = (A ×ˢ B) ∪ (A ×ˢ C) := by sorry
+theorem SetTheory.Set.prod_union (A B C:Set) : A ×ˢ (B ∪ C) = (A ×ˢ B) ∪ (A ×ˢ C) := by
+  ext p
+  constructor
+  . 
+    intro hp
+    rw[mem_cartesian] at hp
+    rw[mem_union,mem_cartesian,mem_cartesian]
+    obtain ⟨x,⟨y,huy⟩ ,hxy⟩ := hp 
+    rw[mem_union] at huy
+    obtain (case|case) := huy
+    map_tacs[left;right]
+    all_goals
+      use x
+      use ⟨y,case⟩ 
+  intro hp
+  rw[mem_union,mem_cartesian,mem_cartesian] at hp
+  rw[mem_cartesian]
+  obtain (⟨x,⟨y,hy⟩ ,p⟩| ⟨x,⟨y,hy⟩ ,p⟩) := hp 
+  all_goals
+    have huy : y ∈ B ∪ C  := by simp[hy]
+    use x, ⟨y,huy⟩ 
 
 /-- Exercise 3.5.4 -/
-theorem SetTheory.Set.prod_inter (A B C:Set) : A ×ˢ (B ∩ C) = (A ×ˢ B) ∩ (A ×ˢ C) := by sorry
+theorem SetTheory.Set.prod_inter (A B C:Set) : A ×ˢ (B ∩ C) = (A ×ˢ B) ∩ (A ×ˢ C) := by
+  ext v
+  rw[mem_cartesian,mem_inter,mem_cartesian,mem_cartesian]
+  constructor
+  . 
+    rintro ⟨x,⟨y,hiy⟩ ,hv⟩  
+    rw[mem_inter] at hiy
+    obtain ⟨hby,hcy⟩ := hiy 
+    split_ands
+    map_tacs[ set y' : B := ⟨y,hby⟩ with hy; set y' : C := ⟨y, hcy⟩with hy]
+    all_goals
+      use x,y'
+  intro ⟨⟨xb,⟨yb,hyb⟩ ,hb⟩ ,⟨xc,⟨yc,hyc⟩ ,hc⟩ ⟩ 
+  rw[hb] at hc
+  simp at hc
+  obtain ⟨hbb, hcc⟩:= hc 
+  have hyi : yb ∈ B ∩ C :=  by
+    aesop
+  use xb, ⟨yb,hyi⟩ 
 
 /-- Exercise 3.5.4 -/
-theorem SetTheory.Set.prod_diff (A B C:Set) : A ×ˢ (B \ C) = (A ×ˢ B) \ (A ×ˢ C) := by sorry
+theorem SetTheory.Set.prod_diff (A B C:Set) : A ×ˢ (B \ C) = (A ×ˢ B) \ (A ×ˢ C) := by
+  ext v
+  rw [mem_cartesian, mem_sdiff,mem_cartesian,mem_cartesian,not_exists]
+  constructor
+  . 
+    rintro ⟨x,⟨y,hy⟩ ,h⟩ 
+    rw[mem_sdiff] at hy
+    obtain ⟨hyb, hyc⟩ := hy 
+    split_ands
+    . use x,⟨y,hyb⟩ 
+    aesop
+  rintro ⟨⟨x,y,hxy⟩ ,h2⟩ 
+  specialize h2 x
+  push_neg at h2
+  aesop
 
 /-- Exercise 3.5.4 -/
-theorem SetTheory.Set.union_prod (A B C:Set) : (A ∪ B) ×ˢ C = (A ×ˢ C) ∪ (B ×ˢ C) := by sorry
+theorem SetTheory.Set.union_prod (A B C:Set) : (A ∪ B) ×ˢ C = (A ×ˢ C) ∪ (B ×ˢ C) := by
+  ext v
+  simp
+  constructor
+  .
+    rintro ⟨x,(hx|hx),y,hyc,hv⟩ 
+    map_tacs[left;right]
+    all_goals
+      use x
+      simp[hx]
+      use y
+
+  rintro (⟨x,hx,y,hy,hv⟩ |⟨x,hx,y,hy,hv⟩) <;> use x <;> split_ands
+  <;> try simp[hx]
+  all_goals
+    use y
 
 /-- Exercise 3.5.4 -/
-theorem SetTheory.Set.inter_prod (A B C:Set) : (A ∩ B) ×ˢ C = (A ×ˢ C) ∩ (B ×ˢ C) := by sorry
-
+theorem SetTheory.Set.inter_prod (A B C:Set) : (A ∩ B) ×ˢ C = (A ×ˢ C) ∩ (B ×ˢ C) := by
+  ext v
+  simp
+  constructor
+  . 
+    rintro ⟨x,⟨hax,hbx⟩,y,hyc,hv ⟩ 
+    split_ands
+    all_goals
+      use x
+      tauto
+  rintro ⟨⟨xa,ha,ya,hyac,hva⟩ ,⟨xb,hb,yb,hybc,hvb⟩ ⟩ 
+  rw[hva] at hvb
+  simp at hvb
+  obtain ⟨hx,hy⟩:= hvb 
+  use xa
+  split_ands
+  . exact ha
+  . rw[hx]; exact hb
+  . use ya
 /-- Exercise 3.5.4 -/
-theorem SetTheory.Set.diff_prod (A B C:Set) : (A \ B) ×ˢ C = (A ×ˢ C) \ (B ×ˢ C) := by sorry
+theorem SetTheory.Set.diff_prod (A B C:Set) : (A \ B) ×ˢ C = (A ×ˢ C) \ (B ×ˢ C) := by
+  ext v
+  simp
+  constructor
+  . 
+    rintro ⟨a,⟨⟨haa,hab⟩ ,⟨c,hc,hv⟩ ⟩ ⟩ 
+    split_ands
+    . 
+      use a
+      simp[haa]
+      use c
+    intro b hb c' hc'
+    rw[hv]
+    simp
+    intro hab'
+    rw[hab'] at hab
+    contradiction
+  rintro ⟨⟨a,ha,c,hc,hv⟩ , hb⟩ 
+  use a
+  by_cases hab : a ∈ B
+  . specialize hb a hab c hc
+    contradiction
+  simp [ha,hab]
+  use c
 
 /-- Exercise 3.5.5 -/
 theorem SetTheory.Set.inter_of_prod (A B C D:Set) :
-    (A ×ˢ B) ∩ (C ×ˢ D) = (A ∩ C) ×ˢ (B ∩ D) := by sorry
+    (A ×ˢ B) ∩ (C ×ˢ D) = (A ∩ C) ×ˢ (B ∩ D) := by
+      ext v
+      simp
+      constructor
+      . 
+        rintro ⟨⟨a,ha,b,hb,hab⟩ ,⟨c,hc,d,hd,hcd⟩ ⟩ 
+        simp[hab]at hcd
+        obtain ⟨hac,hbd⟩ := hcd
+        rw[hac]at ha
+        rw[hbd] at hb
+        use c
+        simp[ha,hc]
+        use d
+        simp[hb,hd]
+        simp[hab,hac,hbd]
+      rintro ⟨x,⟨hxa,hxc⟩ ,y,⟨hyb,hyd⟩,hv ⟩ 
+      split_ands
+      <;> tauto
+
+
 
 /- Exercise 3.5.5 -/
 def SetTheory.Set.union_of_prod :
   Decidable (∀ (A B C D:Set), (A ×ˢ B) ∪ (C ×ˢ D) = (A ∪ C) ×ˢ (B ∪ D)) := by
   -- the first line of this construction should be `apply isTrue` or `apply isFalse`.
-  sorry
+  apply isFalse
+  simp
+  use {0},{1},{2},{3}
+  rw[SetTheory.Set.ext_iff]
+  push_neg
+  use ((⟨0,3⟩ : OrderedPair) : Object)
+  right
+  aesop
 
 /- Exercise 3.5.5 -/
 def SetTheory.Set.diff_of_prod :
   Decidable (∀ (A B C D:Set), (A ×ˢ B) \ (C ×ˢ D) = (A \ C) ×ˢ (B \ D)) := by
   -- the first line of this construction should be `apply isTrue` or `apply isFalse`.
-  sorry
+  apply isFalse
+  simp
+  use {1,2} ,{3,4},{1},{3}
+  rw[SetTheory.Set.ext_iff]
+  push_neg
+  use ((⟨2,3⟩:OrderedPair) : Object) 
+  left
+  simp
 
 /--
   Exercise 3.5.6.
 -/
 theorem SetTheory.Set.prod_subset_prod {A B C D:Set}
   (hA: A ≠ ∅) (hB: B ≠ ∅) (hC: C ≠ ∅) (hD: D ≠ ∅) :
-    A ×ˢ B ⊆ C ×ˢ D ↔ A ⊆ C ∧ B ⊆ D := by sorry
+    A ×ˢ B ⊆ C ×ˢ D ↔ A ⊆ C ∧ B ⊆ D := by
+      rw[subset_def,subset_def,subset_def]
+      constructor 
+      .
+        intro h
+        apply nonempty_def at hA
+        obtain ⟨a,ha⟩ := hA 
+        apply nonempty_def at hB
+        obtain ⟨b,hb⟩ := hB 
+        split_ands
+        <;> intro x hx
+        . 
+          specialize h (⟨x, b⟩ :OrderedPair)
+          simp at h
+          specialize h hx hb
+          exact h.1
+        specialize h (⟨a, x⟩ : OrderedPair)
+        simp at h
+        specialize h ha hx
+        exact h.2
+      rintro ⟨h1, h2⟩ 
+      intro x hx
+      rw[mem_cartesian] at hx ⊢
+      obtain ⟨⟨a,ha⟩ ,⟨b,hb⟩ ,hx ⟩:= hx 
+      simp at hx
+      apply h1 at ha
+      apply h2 at hb
+      use ⟨a,ha⟩, ⟨b, hb⟩  
 
 def SetTheory.Set.prod_subset_prod' :
   Decidable (∀ (A B C D:Set), A ×ˢ B ⊆ C ×ˢ D ↔ A ⊆ C ∧ B ⊆ D) := by
   -- the first line of this construction should be `apply isTrue` or `apply isFalse`.
-  sorry
+  apply isFalse
+  push_neg
+  use  {1} ,∅ ,∅  ,∅  
+  left
+  split_ands
+  . 
+    rw[subset_def]
+    intro x
+    rw[mem_cartesian]
+    rintro ⟨fst,⟨snd,hsnd⟩ ,hx⟩ 
+    simp at hsnd
+  .
+    intro cont
+    rw[subset_def] at cont
+    specialize cont 1
+    simp at cont
+
 
 /-- Exercise 3.5.7 -/
 theorem SetTheory.Set.direct_sum {X Y Z:Set} (f: Z → X) (g: Z → Y) :
-    ∃! h: Z → X ×ˢ Y, fst ∘ h = f ∧ snd ∘ h = g := by sorry
+    ∃! h: Z → X ×ˢ Y, fst ∘ h = f ∧ snd ∘ h = g := by
+      apply existsUnique_of_exists_of_unique
+      . 
+        use fun z ↦  ⟨ (⟨f z, g z⟩:OrderedPair) , by simp⟩ 
+        split_ands
+        all_goals
+          ext z
+          simp
+      intro h1 h2
+      rintro ⟨fh1, gh1⟩ ⟨fh2,gh2⟩ 
+      ext z
+      have eqfst : fst (h1 z) =  fst (h2 z) := by
+        calc 
+          fst (h1 z) = f z := by rw[← fh1, Function.comp_apply]
+          f z = fst (h2 z) := by rw[← fh2, Function.comp_apply]
+      have eqsnd : snd (h1 z) =  snd (h2 z) := by
+        calc 
+          snd (h1 z) = g z := by rw[← gh1, Function.comp_apply]
+          g z = snd (h2 z) := by rw[← gh2, Function.comp_apply]
+      have p1 := mk_cartesian_fst_snd_eq (h1 z)
+      have p2 := mk_cartesian_fst_snd_eq (h2 z)
+      rw[eqfst,eqsnd] at p1
+      rw[p1]at p2
+      congr
+
 
 /-- Exercise 3.5.8 -/
 @[simp]
 theorem SetTheory.Set.iProd_empty_iff {n:ℕ} {X: Fin n → Set} :
-    iProd X = ∅ ↔ ∃ i, X i = ∅ := by sorry
+    iProd X = ∅ ↔ ∃ i, X i = ∅ := by
+      constructor <;> contrapose!
+      . 
+        intro hi
+        let fx : (i : Fin n) → X i := fun i ↦ 
+          ⟨ (nonempty_def (hi i)).choose, (nonempty_def (hi i)).choose_spec ⟩
+        have htup := tuple_mem_iProd fx
+        exact nonempty_of_inhabited htup
+      intro hi
+      replace hi := nonempty_def hi
+      obtain ⟨tup, htup⟩ := hi 
+      rw[mem_iProd] at htup
+      obtain ⟨fx, hfx⟩:= htup 
+      intro i
+      have ⟨xi, hxi⟩  := fx i
+      exact nonempty_of_inhabited hxi
 
 /-- Exercise 3.5.9-/
 theorem SetTheory.Set.iUnion_inter_iUnion {I J: Set} (A: I → Set) (B: J → Set) :
-    (iUnion I A) ∩ (iUnion J B) = iUnion (I ×ˢ J) (fun p ↦ (A (fst p)) ∩ (B (snd p))) := by sorry
+    (iUnion I A) ∩ (iUnion J B) = iUnion (I ×ˢ J) (fun p ↦ (A (fst p)) ∩ (B (snd p))) := by
+      ext v
+      simp[mem_iUnion]
+      constructor
+      .
+        rintro ⟨⟨i,hi,hia⟩ ,⟨j,hj,hjb⟩ ⟩ 
+        use (⟨i,j⟩:OrderedPair )
+        simp
+        use ⟨hi, hj⟩ 
+        rw[fst_of_mk_cartesian ⟨i, hi⟩ ⟨j, hj⟩ ]
+        rw[snd_of_mk_cartesian ⟨i, hi⟩ ⟨j, hj⟩ ]
+        exact ⟨hia, hjb⟩ 
+      rintro ⟨p,⟨a,hai,b,hbj,rfl⟩ ,⟨hvA,hvB⟩ ⟩ 
+      rw[fst_of_mk_cartesian ⟨a, hai⟩ ⟨b, hbj⟩ ] at hvA
+      rw[snd_of_mk_cartesian ⟨a, hai⟩ ⟨b, hbj⟩ ] at hvB
+      split_ands
+      . 
+        use a, hai 
+      use b, hbj
 
 abbrev SetTheory.Set.graph {X Y:Set} (f: X → Y) : Set :=
   (X ×ˢ Y).specify (fun p ↦ (f (fst p) = snd p))
 
 /-- Exercise 3.5.10 -/
 theorem SetTheory.Set.graph_inj {X Y:Set} (f f': X → Y) :
-    graph f = graph f' ↔ f = f' := by sorry
+    graph f = graph f' ↔ f = f' := by
+      rw[SetTheory.Set.ext_iff]
+      constructor
+      .
+        intro h
+        ext x
+        set y := f x with hy
+        symm at hy
+        set y' :=f' x with hy'
+        set p : OrderedPair := ⟨x, y⟩ with hp
+        set p' : OrderedPair  := ⟨x,y'⟩ 
+        specialize h p
+        rw[specification_axiom'',specification_axiom''] at h
+        simp at h
+        specialize h x x.property y y.property hp 
+        have r := h.mp hy
+        rw[← hy'] at r
+        symm at r
+        simp[r]
+      intro hf p
+      rw[specification_axiom'',specification_axiom'']
+      constructor <;> rintro ⟨hp,hfe⟩ <;> use hp
+      map_tacs[rw[← hf]; rw[hf]]
+      assumption'
 
 theorem SetTheory.Set.is_graph {X Y G:Set} (hG: G ⊆ X ×ˢ Y)
   (hvert: ∀ x:X, ∃! y:Y, ((⟨x,y⟩:OrderedPair):Object) ∈ G) :
-    ∃! f: X → Y, G = graph f := by sorry
+    ∃! f: X → Y, G = graph f := by
+      apply existsUnique_of_exists_of_unique
+      . 
+        -- revert the function
+        set fx : X → Y := fun x ↦ (ExistsUnique.exists (hvert x)).choose
+        use fx
+        ext po
+        constructor
+        . 
+          -- prepare the xy pair
+          intro hp
+          have hpu : po ∈ X ×ˢ Y := by
+            rw[subset_def]at hG
+            exact hG po hp
+          set p: X ×ˢ Y := ⟨po,hpu⟩  
+          have:  po =p.val := by rfl
+          rw[this]
+          simp
+          have eq := mk_cartesian_fst_snd_eq p
+          unfold mk_cartesian at eq
+          symm at eq
+          set x := fst p
+          set y := snd p
+          split_ands
+          . 
+            use x, x.property, y, y.property
+            rw[eq]
+          simp[fx]
+          have unique := hvert x
+          have spec := (ExistsUnique.exists (hvert x)).choose_spec
+          rw[this,eq] at hp
+          exact ExistsUnique.unique unique spec hp
+        intro hp
+        have hpu : po ∈ X ×ˢ Y := by
+          exact specification_axiom hp
+        simp[specification_axiom''] at hp
+        obtain ⟨⟨x,hx,y,hy,hpo⟩ , hfx⟩ := hp 
+        set p : X ×ˢ Y := ⟨po, hpu⟩ with hppo
+        have hpx : fst p = x := by
+          have temp := fst_of_mk_cartesian ⟨x, hx⟩ ⟨y, hy⟩ 
+          unfold mk_cartesian at temp
+          simp_all only
+        have hpy : snd p = y := by
+          have temp := snd_of_mk_cartesian ⟨x, hx⟩ ⟨y, hy⟩ 
+          unfold mk_cartesian at temp
+          simp_all only
+        simp[fx] at hfx
+        have unique := hvert (fst p)
+        simp at unique
+        rw[hpo]
+        have spec := (ExistsUnique.exists unique).choose_spec
+        rw[hfx] at spec
+        rw[hpx,hpy] at spec
+        exact spec
+      intro f1 f2 gf1 gf2
+      funext x
+      set y1 := f1 x
+      set y2 := f2 x
+      specialize hvert x
+      apply ExistsUnique.unique hvert
+      . 
+        rw[gf1]
+        simp[specification_axiom'',y1]
+      rw[gf2]
+      simp[specification_axiom'',y2]
+
+
 
 /--
   Exercise 3.5.11. This trivially follows from `SetTheory.Set.powerset_axiom`, but the
   exercise is to derive it from `SetTheory.Set.exists_powerset` instead.
 -/
-theorem SetTheory.Set.powerset_axiom' (X Y:Set) :
-    ∃! S:Set, ∀(F:Object), F ∈ S ↔ ∃ f: Y → X, f = F := sorry
 
+
+theorem SetTheory.Set.powerset_axiom' (X Y:Set) :
+    ∃! S:Set, ∀(F:Object), F ∈ S ↔ ∃ f: Y → X, f = F := by
+      have h_exist_powerset := SetTheory.Set.exists_powerset (Y ×ˢ X)
+      obtain ⟨Z, hZ⟩ := h_exist_powerset 
+
+      -- coe of subset and Z 
+
+      set rv_subset : Z → Set := fun z ↦ 
+        ((hZ z.val).mp z.property).choose
+
+      have rv_Inv (z:Z) : z = set_to_object (rv_subset z) := by
+        simp[rv_subset]
+        exact  ((hZ z.val).mp z.property).choose_spec.1
+
+
+      have subset_spec (z:Z) := ((hZ z.val).mp z.property).choose_spec.2
+
+      -- mapping and function graph 
+      set is_mapping : Z → Prop := fun z ↦ 
+        ∀ y:Y, ∃! x:X, ((⟨y,x⟩: OrderedPair): Object) ∈ rv_subset z
+      have mapping_is_graph (z : Z) : is_mapping z → ∃ f : Y → X, rv_subset z = graph f:= by
+        unfold is_mapping
+        intro hvert
+        have hGSub := subset_spec z
+        have hFun := is_graph hGSub hvert
+        unfold rv_subset
+        exact ExistsUnique.exists hFun
+      have graph_in_Z : ∀ f: Y → X, ((graph f):Object) ∈ Z := by
+        intro f
+        replace hZ := (hZ (graph f)).mpr
+        apply hZ
+        use (graph f)
+        simp
+        apply specification_axiom
+      have rvInv' : ∀ f : Y → X, rv_subset ⟨(graph f), graph_in_Z f⟩ = graph f := by 
+        intro f
+        rw[← coe_eq_iff]
+        symm
+        have inv := rv_Inv (⟨graph f, graph_in_Z f⟩ )
+        rw[← inv]
+
+      have graph_is_mapping : ∀ f: Y → X , is_mapping ⟨graph f, graph_in_Z f⟩ := by
+        intro f
+        unfold is_mapping
+        intro y
+        apply existsUnique_of_exists_of_unique
+        . 
+          use (f y)
+          rw[rvInv']
+          simp
+        intro x1 x2
+        intro hr1 hr2
+        simp[rvInv',specification_axiom''] at hr1 hr2
+        rwa[hr1] at hr2
+
+      set SMap := Z.specify is_mapping
+
+
+      let obtain_function (s : SMap) : Y → X := 
+         ((mapping_is_graph ⟨s.val,specification_axiom s.property⟩ ) ((specification_axiom' _ _).mp s.property )).choose
+      let obtain_function_spec (s:SMap) :=
+         ((mapping_is_graph ⟨s.val,specification_axiom s.property⟩ ) ((specification_axiom' _ _).mp s.property )).choose_spec
+      
+
+      let rep_prop: SMap → Object → Prop := fun s f ↦ f = obtain_function s
+      set S := SMap.replace (P := rep_prop) (
+        by
+        intro s f1 f2 ⟨pf1,pf2⟩ 
+        simp[rep_prop] at pf1 pf2
+        rw[← pf1]at pf2
+        exact pf2.symm
+      )
+
+      -- finally start to prove unique exists
+      apply existsUnique_of_exists_of_unique 
+      .
+        use S
+        intro F
+        rw[replacement_axiom]
+        unfold rep_prop
+        constructor
+        .
+          intro hF
+          obtain ⟨z,hprop⟩  := hF
+          symm at hprop
+          use (obtain_function z)
+        rintro ⟨f,hf⟩ 
+        set smap : SMap := ⟨graph f, 
+          by
+            rw[specification_axiom'']
+            use (graph_in_Z f)
+            apply graph_is_mapping
+        ⟩ 
+        use smap
+        have spec := obtain_function_spec smap
+        unfold obtain_function
+        simp[← hf,← graph_inj, ← spec]
+        rw[← coe_eq_iff, ← rv_Inv]
+      intro S1 S2 hS1 hS2
+      ext F
+      specialize hS1 F
+      specialize hS2 F
+      simp[hS1,hS2]
+  
 /-- Exercise 3.5.12, with errata from web site incorporated -/
+lemma SetTheory.Set.nat_ind { P : nat → Prop } (pzero : P (nat_equiv 0))  (psucc : (∀ n, P (nat_equiv n) → P (nat_equiv (n+1)))) : ∀ n, P (nat_equiv n) := by
+  intro n
+  induction' n with k hk
+  . 
+    exact pzero
+  apply psucc k hk
+
 theorem SetTheory.Set.recursion (X: Set) (f: nat → X → X) (c:X) :
-    ∃! a: nat → X, a 0 = c ∧ ∀ n, a (n + 1:ℕ) = f n (a n) := by sorry
+    ∃! a: nat → X, a 0 = c ∧ ∀ n, a (n + 1:ℕ) = f n (a n) := by
+      let a : nat → X := fun n ↦ 
+        Nat.rec c (fun n pr ↦ f n pr) n
+      apply existsUnique_of_exists_of_unique
+      .
+        use a
+        simp[a]
+      . 
+        intro a1 a2 ⟨az1, as1⟩ ⟨az2,as2⟩  
+        set P : nat → Prop := fun n ↦ a1 n = a2 n with hp
+        have aux : ∀ n, P (nat_equiv n) := by
+          apply nat_ind
+          . 
+            unfold P
+            have : nat_equiv 0 = 0 := by rfl
+            simp[this,az1,az2]
+          .
+            intro n
+            specialize as1 n
+            specialize as2 n
+            unfold P
+            intro hi
+            have : nat_equiv n = ↑n := by rfl
+            simp[this] at hi
+            rw[hi]at as1
+            rw[← as1] at as2
+            have : nat_equiv (n+1) = ↑(n+1) := by rfl
+            rw[this]
+            exact as2.symm
+        ext n'
+        unfold P at aux
+        set n:= nat_equiv.symm n'
+        specialize aux n
+        have:  nat_equiv n = n' := by simp[n]
+        rw[this] at aux
+        simp[aux]
 
 /-- Exercise 3.5.13 -/
 theorem SetTheory.Set.nat_unique (nat':Set) (zero:nat') (succ:nat' → nat')
@@ -505,15 +1355,44 @@ theorem SetTheory.Set.nat_unique (nat':Set) (zero:nat') (succ:nat' → nat')
     ∧ ∀ (n:nat) (n':nat'), f n = n' ↔ f (n+1:ℕ) = succ n' := by
   have nat_coe_eq {m:nat} {n} : (m:ℕ) = n → m = n := by aesop
   have nat_coe_eq_zero {m:nat} : (m:ℕ) = 0 → m = 0 := nat_coe_eq
-  obtain ⟨f, hf⟩ := recursion nat' sorry sorry
+  obtain ⟨f, hf⟩ := recursion nat' (fun _ n ↦ succ n) zero
   apply existsUnique_of_exists_of_unique
   · use f
     constructor
     · constructor
       · intro x1 x2 heq
         induction' hx1: (x1:ℕ) with i ih generalizing x1 x2
-        · sorry
-        sorry
+        · 
+          simp at hf
+          obtain ⟨⟨hfz,hfi⟩ , hfunique⟩ := hf
+          apply nat_coe_eq_zero at hx1
+          simp[hx1,hfz] at heq
+          rw[hx1]
+          by_contra hnz
+          set x2' :ℕ := (nat_equiv.symm x2)  with hxp
+          have hx2nz : x2' ≠ 0 := by
+            by_contra h
+            rw[hxp] at h
+            have := nat_coe_eq_zero h
+            symm at this
+            contradiction
+          have hx2g1 : 1 ≤ x2' := Nat.succ_le_of_lt (Nat.pos_of_ne_zero hx2nz)
+          have : x2' - 1 + 1 = x2' := by
+            simpa using Nat.sub_add_cancel hx2g1
+          specialize hfi (x2'-1)
+          rw[this] at hfi
+          simp[x2'] at hfi
+          rw[← heq] at hfi
+          symm at hfi
+          specialize succ_ne (f ↑(nat_equiv.symm x2 - 1))
+          contradiction
+
+
+        
+
+
+
+        
       sorry
     sorry
   sorry
